Dom.lean
@@ -59,6 +59,8 @@ import Dom.Properties.Clone
 import Dom.Mutation.Import
 import Dom.Properties.Import
 import Dom.Properties.CloneOk
+import Dom.Attribute.Node
+import Dom.Validity.AttrNode
 import Dom.Spec.Remove
 import Dom.Spec.RemoveSound
 import Dom.Spec.RemoveDeterministic
